Source/Core/set_size.bpl
@@ -1,6 +1,6 @@
 function Set_Size<T>(a: Set T) : int;
 
-axiom (forall<T> a: Set T :: a == Set_Empty() || 0 < Set_Size(a));
+axiom (forall<T> a: Set T :: 0 <= Set_Size(a));
 
 axiom (forall<T> :: Set_Size(Set_Empty(): Set T) == 0);
 
@@ -8,14 +8,22 @@ axiom (forall<T> a: Set T, t: T :: {Set_Add(a, t)} Set_Size(Set_Add(a, t)) == if
 
 axiom (forall<T> a: Set T, t: T :: {Set_Remove(a, t)} Set_Size(Set_Remove(a, t)) == if Set_Contains(a, t) then Set_Size(a) - 1 else Set_Size(a));
 
-axiom (forall<T> a: Set T, b: Set T ::
-        {Set_Difference(a, b)} {Set_Intersection(a, b)} {Set_Union(a, b)}
+axiom (forall<T> a: Set T, b: Set T :: {Set_Size(Set_Difference(a, b))} {Set_Size(Set_Intersection(a, b))}
         Set_Size(a) == Set_Size(Set_Difference(a, b)) + Set_Size(Set_Intersection(a, b)));
 
-axiom (forall<T> a: Set T, b: Set T ::
-        {Set_Union(a, b)} {Set_Intersection(a, b)}
+axiom (forall<T> a: Set T, b: Set T :: {Set_Size(Set_Union(a, b))} {Set_Size(Set_Intersection(a, b))}
         Set_Size(Set_Union(a, b)) + Set_Size(Set_Intersection(a, b)) == Set_Size(a) + Set_Size(b));
 
-pure procedure Lemma_SubsetSize<T>(a: Set T, b: Set T);
+pure procedure Lemma_SetSize_Add<T>(a: Set T, t: T) returns (b: Set T);
+requires !Set_Contains(a, t);
+ensures b == Set_Add(a, t);
+ensures Set_Size(b) == Set_Size(a) + 1;
+
+pure procedure Lemma_SetSize_Remove<T>(a: Set T, t: T) returns (b: Set T);
+requires Set_Contains(a, t);
+ensures b == Set_Remove(a, t);
+ensures Set_Size(b) + 1 == Set_Size(a);
+
+pure procedure Lemma_SetSize_Subset<T>(a: Set T, b: Set T);
 requires Set_IsSubset(a, b);
 ensures a == b || Set_Size(a) < Set_Size(b);
